policy_proof/coq/formula.v
@@ -2,6 +2,11 @@ Require Import types.
 Require Import data_model.
 Require Import ordering.
 
+(*
+  One thing in the relational algbera is that the variables aren't explicitly typed, but in Coq, we need to
+  give types to each expressions. This is the gap. So we need `simple_` versions which are not typed.
+*)
+
 Inductive atomic_expression (ty: Tuple.tuple_type) : basic_type -> Set :=
   (* v *)
   | atomic_expression_const:
@@ -9,7 +14,17 @@ Inductive atomic_expression (ty: Tuple.tuple_type) : basic_type -> Set :=
   (* a *)
   | atomic_expression_column:
       forall n (extract: n < length ty), atomic_expression ty (Tuple.nth_np ty n extract)
+  (* more -> apply function. *)
 .
+
+Inductive simple_atomic_expression: Set :=
+  (* v *)
+  | simple_atomic_expression_const:
+      forall bt (c : type_to_coq_type bt), simple_atomic_expression
+  (* a *)
+  | simple_atomic_expression_column:
+      forall (n: nat), simple_atomic_expression
+  .
 
 Inductive predicate (ty: Tuple.tuple_type) (t: basic_type): Type :=
   | predicate_true: predicate ty t
@@ -18,12 +33,12 @@ Inductive predicate (ty: Tuple.tuple_type) (t: basic_type): Type :=
   | predicate_not: predicate ty t -> predicate ty t
 .
 
-Inductive simple_predicate (bt: basic_type): Set :=
-  | simple_predicate_true: simple_predicate bt
-  | simple_predicate_false: simple_predicate bt
+Inductive simple_predicate: Set :=
+  | simple_predicate_true: simple_predicate
+  | simple_predicate_false: simple_predicate
   (* cell ? basic_type *)
-  | simple_predicate_com: ComOp -> (type_to_coq_type bt) -> simple_predicate bt
-  | simple_predicate_not: simple_predicate bt -> simple_predicate bt
+  | simple_predicate_com: ComOp -> simple_atomic_expression -> simple_atomic_expression -> simple_predicate
+  | simple_predicate_not: simple_predicate -> simple_predicate
 .
 
 Inductive formula (ty: Tuple.tuple_type) :=
@@ -31,9 +46,9 @@ Inductive formula (ty: Tuple.tuple_type) :=
   | formula_predicate: forall bt, predicate ty bt -> formula ty
 .
 
-Inductive simple_formula (bt: basic_type) :=
-  | simple_formula_con: LogOp -> simple_formula bt -> simple_formula bt -> simple_formula bt
-  | simple_formula_predicate: simple_predicate bt -> simple_formula bt
+Inductive simple_formula :=
+  | simple_formula_con: LogOp -> simple_formula -> simple_formula -> simple_formula
+  | simple_formula_predicate: simple_predicate -> simple_formula
 .
 
 Definition atomic_expression_denote (ty: Tuple.tuple_type) (t: basic_type) (a: atomic_expression ty t):
@@ -85,13 +100,13 @@ Fixpoint predicate_denote (bt: basic_type) (ty: Tuple.tuple_type) (p: predicate 
       * exact true.
   - rename H into tp. exact (negb (predicate_denote bt ty p tp)).
 Defined.
-
+(* 
 Fixpoint simple_predicate_denote (bt: basic_type) (p: simple_predicate bt): type_to_coq_type bt -> bool.
   intros. destruct p.
   - exact true.
   - exact false.
   (* Inductive ComOp: Type := Gt | Lt | Ge | Le | Eq | Neq.*)
-  - destruct c; rename t into lhs; rename H into rhs; destruct (cmp lhs rhs).
+  - destruct c. destruct (cmp lhs rhs).
       * exact false.
       * exact false.
       * exact true.
@@ -116,7 +131,7 @@ Fixpoint simple_predicate_denote (bt: basic_type) (p: simple_predicate bt): type
       * exact false.
       * exact true.
   - exact (negb (simple_predicate_denote bt p H)).
-Defined.
+Defined. *)
 
 Fixpoint formula_denote (ty: Tuple.tuple_type) (f: formula ty) {struct f}: Tuple.tuple ty -> bool :=
 match f with
@@ -183,15 +198,3 @@ Proof.
   - reflexivity.
 Qed.
 
-Require Import ordering.
-Example simple_cell := ("abcd"%string, Policy.policy_bot).
-Example simple_predicate': simple_predicate StringType :=
-  simple_predicate_com StringType Eq "abcd"%string.
-
-Definition result:= simple_predicate_denote StringType simple_predicate'.
-
-Lemma result_is_true: result (fst simple_cell) = true.
-Proof.
-  simpl. unfold result. unfold simple_predicate'. unfold simple_predicate_denote.
-  destruct (cmp _ _); str_eq.
-Qed.
