policy_proof/coq/query.v
@@ -1,16 +1,32 @@
+Require Import List.
 Require Import String.
 
 Require Import types.
+Require Import relation.
+Require Import formula.
+Require Import data_model.
 
-Inductive Query: Type :=
-  (* Relation *)
-  | QueryRel : string -> Query
-  (* Union *)
-  | QueryUnion : Query -> Query -> Query
-  (* (Natural) Join *)
-  | QueryJoin : Query -> Query -> Query
-  (* GroupBy and Aggregation *)
-  | QueryGroupBy : Query -> Query -> Query
-  (* Selection *).
+Definition project_list : Set := list simple_atomic_expression%type.
 
+Fixpoint bounded_list (proj: project_list) (ty: Tuple.tuple_type) : Prop :=
+  match proj with
+    | nil => True
+    | h :: t => match h with
+                  | simple_atomic_expression_column n => n < List.length ty
+                  | _ => True
+                end /\ bounded_list t ty
+  end.
 
+Inductive Query: schema -> Set :=
+  | query_empty: forall s, Query s
+  | query_relation: forall s, relation s -> Query s
+  | query_union: forall s, Query s -> Query s -> Query s
+  | query_join: forall s1 s2, Query s1 -> Query s2 -> Query (s1 ++ s2)
+  | query_project:
+      forall s (proj: project_list) (bounded: bounded_list proj (schema_denote s)),
+        Query s -> Query s
+  | query_select:
+    forall s (where_exp: simple_formula), Query s -> Query s
+  (* TODO: Design `groupby`. *)
+  | query_grouby_agg: forall s, Query s -> Query s
+  .
