policy_proof/coq/relation.v
@@ -7,20 +7,43 @@ Require Import ordering.
 Require Import finite_bags.
 Require Import types.
 
+Definition schema_denote (s: schema): Tuple.tuple_type := List.map (fun x => (fst x)) s.
+
 (** 
   [relation_np] is a function that takes a tuple type [ty] as an argument and returns a finite bag (fbag) of tuples of type [ty]. 
   This function is used to define a relation in the context of a database or a similar data structure where relations are represented as collections of tuples.
   Note: this will make tuple ignorant of the policy.
-  @param ty  The type of the tuples that will be stored in the relation.
+  @param s   The schema of the relation.
   @return    A finite bag (fbag) of tuples of type [ty].
 *)
-Definition relation_np (ty: Tuple.tuple_type) := fbag (Tuple.tuple ty).
+Definition relation_np (s: schema) := fbag (Tuple.tuple_np (schema_denote s)).
 
 (** 
   [relation] is a function that takes a tuple type [ty] as an argument and returns a finite bag (fbag) of tuples of type [ty]. 
   This function is used to define a relation in the context of a database or a similar data structure where relations are represented as collections of tuples.
 
-  @param ty  The type of the tuples that will be stored in the relation.
+  @param s   The schema of the relation.
   @return    A finite bag (fbag) of tuples of type [ty].
 *)
-Definition relation (ty: Tuple.tuple_type) := fbag (Tuple.tuple ty).
+Definition relation (s: schema) := fbag (Tuple.tuple (schema_denote s)).
+
+(**
+  [inject_tuple_id_relation] is a function that takes a tuple type [ty], a relation [r] of type [relation_np ty] and an id [id] as arguments and returns a relation of type [relation ty].
+  This function is used to inject an id into a relation. This is useful when we want to inject a policy into a relation.
+  @param s   The schema of the relation that we want to inject an id into.
+  @param r   The relation that we want to inject an id into.
+  @param id  The id that we want to inject into the relation.
+  @return    A relation of type [relation ty].
+*)
+Fixpoint inject_tuple_id_relation
+  (s: schema)
+  (r: relation_np s)
+  (id: nat)
+: relation s :=
+  match r with
+  | nil => nil
+  | cons t r' =>
+    let ty := (schema_denote s) in
+      cons (Tuple.inject_tuple_id ty t id) (inject_tuple_id_relation s r' (id + List.length ty))
+  end.
+
